ArrayList con la nueva interfaz unificada

src/linear/layer3/ArrayListImpl.dfy
@@ -6,78 +6,112 @@ class ArrayListIteratorImpl<A> extends ListIterator<A> {
   var parent: ArrayListImpl<A>
   var index: nat
 
+  function Parent(): List<A>
+    reads this
+  { parent }
+
   predicate Valid()
-    reads this, parent, parent.Repr()
+    reads this, Parent(), Parent().Repr()
+    ensures Valid() ==> Parent().Valid() && this in Parent().Iterators()
   {
-    parent.Valid()
+    Parent().Valid()
+    && this in Parent().Iterators()
     && 0 <= index <= parent.size
   }
 
-  function Parent(): List<A>
-    reads this
-  {
-    parent
-  }
-
   function Index() : nat
-    reads this, parent, parent.Repr()
+    reads this, Parent(), Parent().Repr()
     requires Valid()
     requires Parent().Valid()
     ensures Index() <= |Parent().Model()|
-  {
-    index
-  }
+  { index }
 
-  constructor(vector: ArrayListImpl<A>)
-    requires vector.Valid()
+  constructor(parent: ArrayListImpl<A>)
+    modifies parent
+    requires parent.Valid()
     ensures Valid()
-    ensures Parent() == vector
+    ensures Parent() == parent
     ensures Index() == 0
+    ensures parent.iterators == old(parent.iterators) + { this }
+    ensures parent.Model() == old(parent.Model())
+    ensures fresh(parent.Repr() - old(parent.Repr()))
   {
-    this.parent := vector;
+    this.parent := parent;
     this.index := 0;
+    new;
+    this.parent.iterators := this.parent.iterators + { this };
   }
 
-  function method HasNext(): bool
-    reads this, Parent(), Parent().Repr()
+  method HasNext() returns (b: bool) 
+    modifies this, Parent(), Parent().Repr()
+    requires allocated(Parent())
+    requires allocated(Parent().Repr())
+    
     requires Valid()
     requires Parent().Valid()
-    ensures HasNext() <==> Index() < |Parent().Model()|
+    ensures Valid()
+    ensures Parent().Valid()
+    ensures Parent() == old(Parent())
+    ensures Parent().Model() == old(Parent().Model()) 
+    ensures Index() == old(Index())
+    ensures b == HasNext?()
+
+    ensures fresh(Parent().Repr() - old(Parent().Repr()))
+    ensures allocated(Parent().Repr())
+
+    ensures Parent().Iterators() >= old(Parent().Iterators())
+    ensures forall it | it in old(Parent().Iterators()) && old(it.Valid()) ::
+      it.Valid() && it.Parent() == old(it.Parent()) && it.Index() == old(it.Index())
   {
-    index < parent.size
+    b := index < parent.size;
   }
 
-  function method Peek(): A
-    reads this, Parent(), Parent().Repr()
+  method Peek() returns (p: A)
+    modifies this, Parent(), Parent().Repr()
+    requires allocated(Parent())
+    requires allocated(Parent().Repr())
+    
     requires Valid()
     requires Parent().Valid()
-    requires HasNext()
-    ensures Peek() == Parent().Model()[Index()]
+    requires HasNext?()
+    ensures Valid()
+    ensures Parent().Valid()
+    ensures Parent() == old(Parent())  
+    ensures Parent().Model() == old(Parent().Model())  
+    ensures Index() == old(Index())
+    ensures p == Parent().Model()[Index()] 
+    
+    ensures fresh(Parent().Repr() - old(Parent().Repr()))
+    ensures allocated(Parent().Repr())
+
+    ensures Parent().Iterators() >= old(Parent().Iterators())
+    ensures forall it | it in old(Parent().Iterators()) && old(it.Valid()) ::
+      it.Valid() && it.Parent() == old(it.Parent()) && it.Index() == old(it.Index())
   {
-    parent.elements[index]
+    p := parent.elements[index];
   }
 
   method Next() returns (x: A)
-    modifies this
+    modifies this, Parent(), Parent().Repr()
+    requires allocated(Parent())
+    requires allocated(Parent().Repr())
+    
     requires Valid()
     requires Parent().Valid()
-    requires HasNext()
-    requires allocated(Parent())
-    requires forall it | it in Parent().Repr() :: allocated(it)
-    ensures Parent().Valid()
+    requires HasNext?()
     ensures Valid()
-    ensures old(Parent()) == Parent()
-    ensures old(Parent().Model()) == Parent().Model()       // ?
+    ensures Parent().Valid()
+    ensures Parent() == old(Parent())  
+    ensures Parent().Model() == old(Parent().Model())  
 
-    ensures forall x {:trigger x in Parent().Repr(), x in old(Parent().Repr())} | x in Parent().Repr() - old(Parent().Repr()) :: fresh(x)
     ensures fresh(Parent().Repr() - old(Parent().Repr()))
-    ensures forall x | x in Parent().Repr() :: allocated(x)
+    ensures allocated(Parent().Repr())
 
-    ensures Parent().Iterators() == old(Parent().Iterators())   // ?
+    ensures Parent().Iterators() >= old(Parent().Iterators())
     ensures x == Parent().Model()[old(Index())]
     ensures Index() == 1 + old(Index())
-    ensures forall it | it in Parent().Iterators() && old(it.Valid()) ::
-       it.Valid() && (it != this ==> it.Index() == old(it.Index()))
+    ensures forall it | it in old(Parent().Iterators()) && old(it.Valid()) ::
+      it.Valid() && it.Parent() == old(it.Parent()) && (it != this ==> it.Index() == old(it.Index()))
     {
       var elem := parent.elements[index];
       index := index + 1;
@@ -85,27 +119,28 @@ class ArrayListIteratorImpl<A> extends ListIterator<A> {
     }
 
   method Copy() returns (it: ListIterator<A>)
-    modifies Parent(), Parent().Repr()
+    modifies this, Parent(), Parent().Repr()
+    requires allocated(Parent())
+    requires allocated(Parent().Repr())
+    
     requires Valid()
     requires Parent().Valid()
-    requires allocated(Parent())
-    requires forall it | it in Parent().Iterators() :: allocated(it)
     ensures fresh(it)
     ensures Valid()
-    ensures Parent() == old(Parent())
     ensures Parent().Valid()
+    ensures Parent() == old(Parent())
     ensures Parent().Model() == old(Parent().Model())
+    ensures Index() == old(Index())
 
-    ensures forall x {:trigger x in Parent().Repr(), x in old(Parent().Repr())} | x in Parent().Repr() - old(Parent().Repr()) :: fresh(x)
-    ensures fresh(Parent().Repr()-old(Parent().Repr()))
-    ensures forall x | x in Parent().Repr() :: allocated(x)
+    ensures fresh(Parent().Repr() - old(Parent().Repr()))
+    ensures allocated(Parent().Repr())
     
     ensures it.Valid()
-    ensures Parent().Iterators() == {it} + old(Parent().Iterators())
+    ensures Parent().Iterators() >= {it} + old(Parent().Iterators())
     ensures Parent() == it.Parent()
     ensures Index() == it.Index()
     ensures forall it | it in old(Parent().Iterators()) && old(it.Valid()) ::
-      it.Valid() && it.Index() == old(it.Index())
+      it.Valid() && it.Parent() == old(it.Parent()) && it.Index() == old(it.Index())
     {
       var itImpl := new ArrayListIteratorImpl(parent);      
       itImpl.index := index;
@@ -114,28 +149,26 @@ class ArrayListIteratorImpl<A> extends ListIterator<A> {
     }
 
   method Set(x: A)
-    modifies Parent(), Parent().Repr()
+    modifies this, Parent(), Parent().Repr()
+    requires allocated(Parent())
+    requires allocated(Parent().Repr())
+   
     requires Valid()
     requires Parent().Valid()
-    requires allocated(Parent())
-    requires forall it | it in Parent().Repr() :: allocated(it)
-    requires HasNext()
+    requires HasNext?()
     ensures Valid()
     ensures Parent().Valid()
     ensures Parent() == old(Parent())
     ensures |Parent().Model()| == old(|Parent().Model()|)
-    ensures Parent().Model()[old(Index())] == x
-    ensures forall i | 0 <= i < |Parent().Model()| && i != old(Index()) ::
-      Parent().Model()[i] == old(Parent().Model()[i])
+    ensures Index() == old(Index()) 
+    ensures Parent().Model() == old(Parent().Model()[Index():=x])
+    
+    ensures fresh(Parent().Repr() - old(Parent().Repr()))
+    ensures allocated(Parent().Repr())
 
-    ensures forall x {:trigger x in Parent().Repr(), x in old(Parent().Repr())} | x in Parent().Repr() - old(Parent().Repr()) :: fresh(x)
-    ensures fresh(Parent().Repr()-old(Parent().Repr()))
-    ensures forall x | x in Parent().Repr() :: allocated(x)
-
-    //ensures Index() == old(Index())
-    ensures Parent().Iterators() == old(Parent().Iterators())
+    ensures Parent().Iterators() >= old(Parent().Iterators())
     ensures forall it | it in old(Parent().Iterators()) && old(it.Valid()) ::
-      it.Valid() && it.Index() == old(it.Index())
+      it.Valid() && it.Parent() == old(it.Parent()) && it.Index() == old(it.Index())
  {
     parent.elements[index] := x;
   }
@@ -199,50 +232,74 @@ class ArrayListImpl<A> extends ArrayList<A> {
     iterators := {};
   }
 
-  function method Empty(): bool
-    reads this, Repr()
-    requires Valid()
-    ensures Empty() <==> Model() == []
-  {
-    size == 0
-  }
-
-
-  function method Size(): nat
-    reads this, Repr()
-    requires Valid()
-    ensures Size() == |Model()|
-  {
-    size
-  }
-
-
-  function method Front(): A
-    reads this, Repr()
-    requires Valid()
-    requires Model() != []
+  method Empty() returns (b: bool)
+    modifies this, Repr()
+    requires allocated(Repr())
     
+    requires Valid()
     ensures Valid()
-    ensures Front() == Model()[0]
+    ensures Model() == old(Model())
+    ensures b == Empty?() 
+
+    ensures fresh(Repr() - old(Repr()))
+    ensures allocated(Repr())
+ 
+    ensures Iterators() >= old(Iterators())
   {
-    elements[0]
+    b := size == 0;
+  }
+
+
+  method Size() returns (s: int)
+    modifies this, Repr()
+    requires allocated(Repr())
+    
+    requires Valid()
+    ensures Valid()
+    ensures Model() == old(Model())
+    ensures s == |Model()| 
+
+    ensures fresh(Repr() - old(Repr()))
+    ensures allocated(Repr())
+
+    ensures Iterators() >= old(Iterators())
+  {
+    s := size;
+  }
+
+
+  method Front() returns (x: A)
+    modifies this, Repr()
+    requires allocated(Repr())
+    
+    requires Valid()
+    requires !Empty?()
+    ensures Valid()
+    ensures Model() == old(Model())
+    ensures x == Model()[0]
+
+    ensures fresh(Repr() - old(Repr()))
+    ensures allocated(Repr())
+ 
+    ensures Iterators() >= old(Iterators())
+  {
+    x := elements[0];
   }
 
   method PushFront(x: A)
     modifies this, Repr()
-    requires Valid()
-    requires forall x | x in Repr() :: allocated(x)
+    requires allocated(Repr())
     
+    requires Valid()
     ensures Valid()
     ensures Model() == [x] + old(Model())
 
-    ensures forall x {:trigger x in Repr(), x in old(Repr())} | x in Repr() - old(Repr()) :: fresh(x)
     ensures fresh(Repr() - old(Repr()))
-    ensures forall x | x in Repr() :: allocated(x)
+    ensures allocated(Repr())
 
-    ensures Iterators() == old(Iterators())
-    ensures forall it | it in old(Iterators()) && old(it.Valid())
-      :: it.Valid() && old(it.Parent()) == it.Parent() && old(it.Index()) == it.Index();
+    ensures Iterators() >= old(Iterators())
+    ensures forall it | it in old(Iterators()) && old(it.Valid()) ::
+      it.Valid() && it.Parent() == old(it.Parent()) && it.Index() == old(it.Index())
   {      
     if (size == elements.Length) {
       Grow(elements.Length * 2 + 1, x);
@@ -255,53 +312,58 @@ class ArrayListImpl<A> extends ArrayList<A> {
 
   method PopFront() returns (x: A)
     modifies this, Repr()
+    requires allocated(Repr())
+   
     requires Valid()
-    requires Model() != []
-    requires forall x | x in Repr() :: allocated(x)
-
+    requires !Empty?()
     ensures Valid()
     ensures [x] + Model() == old(Model())
 
-    ensures forall x {:trigger x in Repr(), x in old(Repr())} | x in Repr() - old(Repr()) :: fresh(x)
     ensures fresh(Repr() - old(Repr()))
-    ensures forall x | x in Repr() :: allocated(x)
+    ensures allocated(Repr())
 
-    ensures Iterators() == old(Iterators())
-    ensures forall it | it in old(iterators) && old(it.Valid()) && old(it.HasNext())
-      :: it.Valid() && old(it.Parent()) == it.Parent() && old(it.Index()) == it.Index();
+    ensures Iterators() >= old(Iterators())
+    ensures forall it | it in old(Iterators()) && old(it.Valid()) && old(it.HasNext?())
+      :: it.Valid() && it.Parent() == old(it.Parent()) && it.Index() == old(it.Index())
   {
     x := elements[0];
     ShiftLeft(0);
     size := size - 1;
   }
 
-  function method Back(): A
-    reads this, Repr()
-    requires Valid()
-    requires Model() != []
+  method Back() returns (x: A)//Nuevo metodo
+    modifies this, Repr()
+    requires allocated(Repr())
     
+    requires Valid()
+    requires !Empty?()
     ensures Valid()
-    ensures Back() == Model()[|Model()|-1]
+    ensures Model() == old(Model())
+    ensures x == Model()[|Model()| - 1]
+
+    ensures fresh(Repr() - old(Repr()))
+    ensures allocated(Repr())
+ 
+    ensures Iterators() >= old(Iterators())
   {
-    elements[size - 1]
+    x := elements[size - 1];
   }
 
   method PopBack() returns (x: A)
     modifies this, Repr()
-    requires Valid()
-    requires Model() != []
-    requires forall x | x in Repr() :: allocated(x)
+    requires allocated(Repr())
     
+    requires Valid()
+    requires !Empty?()
     ensures Valid()
     ensures Model() + [x] == old(Model())
 
-    ensures forall x {:trigger x in Repr(), x in old(Repr())} | x in Repr() - old(Repr()) :: fresh(x)
     ensures fresh(Repr() - old(Repr()))
-    ensures forall x | x in Repr() :: allocated(x)
+    ensures allocated(Repr())
 
-    ensures Iterators() == old(Iterators())
-    ensures forall it | it in old(Iterators()) && old(it.Valid()) && old(it.HasNext())
-      :: it.Valid() && old(it.Parent()) == it.Parent() && old(it.Index()) == it.Index();
+    ensures Iterators() >= old(Iterators())
+    ensures forall it | it in old(Iterators()) && old(it.Valid()) && old(it.HasNext?())
+      :: it.Valid() && it.Parent() == old(it.Parent()) && it.Index() == old(it.Index())
   {
     assert size > 0;
     x := elements[size - 1];
@@ -311,19 +373,18 @@ class ArrayListImpl<A> extends ArrayList<A> {
 
   method PushBack(x: A)
     modifies this, Repr()
-    requires Valid()
-    requires forall x | x in Repr() :: allocated(x)
+    requires allocated(Repr())
     
+    requires Valid()
     ensures Valid()
     ensures Model() == old(Model()) + [x]
 
-    ensures forall x {:trigger x in Repr(), x in old(Repr())} | x in Repr() - old(Repr()) :: fresh(x)
     ensures fresh(Repr() - old(Repr()))
-    ensures forall x | x in Repr() :: allocated(x)
+    ensures allocated(Repr())
 
-    ensures Iterators() == old(Iterators())
-    ensures forall it | it in old(iterators) && old(it.Valid())
-      :: it.Valid() && old(it.Parent()) == it.Parent() && old(it.Index()) == it.Index();
+    ensures Iterators() >= old(Iterators())
+    ensures forall it | it in old(Iterators()) && old(it.Valid())
+      :: it.Valid() && it.Parent() == old(it.Parent()) && it.Index() == old(it.Index())
   {
     if (size == elements.Length) {
       Grow(elements.Length * 2 + 1, x);
@@ -335,23 +396,22 @@ class ArrayListImpl<A> extends ArrayList<A> {
 
   method Begin() returns (it: ListIterator<A>)
     modifies this, Repr()
-    requires Valid()
-    requires forall x | x in Repr()::allocated(x)
+    requires allocated(Repr())
     
+    requires Valid()
     ensures Valid()
     ensures Model() == old(Model())
 
-    ensures forall x {:trigger x in Repr(), x in old(Repr())} | x in Repr() - old(Repr()) :: fresh(x)
     ensures fresh(Repr() - old(Repr()))
-    ensures forall x | x in Repr() :: allocated(x)
+    ensures allocated(Repr())
 
     ensures fresh(it)
+    ensures Iterators() >= {it} + old(Iterators())
     ensures it.Valid()
-    ensures it.Parent() == this
     ensures it.Index() == 0
-    ensures Iterators() == {it} + old(Iterators())
-    ensures forall it | it in old(Iterators()) && old(it.Valid())
-      :: it.Valid() && old(it.Parent()) == it.Parent() && old(it.Index()) == it.Index();
+    ensures it.Parent() == this
+    ensures forall it | it in old(Iterators()) && old(it.Valid()) ::
+      it.Valid() && it.Parent() == old(it.Parent()) && it.Index() == old(it.Index())
   {
     it := new ArrayListIteratorImpl(this);
     iterators := iterators + { it };
@@ -360,25 +420,24 @@ class ArrayListImpl<A> extends ArrayList<A> {
   // Deletion of mid, next points to the next element (or past-the-end)
   method Insert(mid: ListIterator<A>, x: A) returns (newt: ListIterator<A>)
     modifies this, Repr()
+    requires allocated(Repr())
+
     requires Valid()
     requires mid.Valid()
     requires mid.Parent() == this
     requires mid in Iterators()
-    requires forall x | x in Repr() :: allocated(x)
-
     ensures Valid()
     ensures Model() == Seq.Insert(x, old(Model()), old(mid.Index()))
 
-    ensures forall x {:trigger x in Repr(), x in old(Repr())} | x in Repr() - old(Repr()) :: fresh(x)
     ensures fresh(Repr() - old(Repr()))
-    ensures forall x | x in Repr() :: allocated(x)
+    ensures allocated(Repr())
 
     ensures fresh(newt)
-    ensures Iterators() == {newt}+old(Iterators())
-    ensures newt.Valid() && newt.Parent()==this && newt.Index()==old(mid.Index())
-    
+    ensures Iterators() >= {newt} + old(Iterators())
+    ensures newt.Valid() && newt.Parent() == this && newt.Index() == old(mid.Index())
+ 
     ensures forall it | it in old(Iterators()) && old(it.Valid())
-      :: it.Valid() && old(it.Parent()) == it.Parent() && old(it.Index()) == it.Index();
+      :: it.Valid() && it.Parent() == old(it.Parent()) && it.Index() == old(it.Index())
   {
     var midImpl := mid as ArrayListIteratorImpl;
    
@@ -403,25 +462,24 @@ class ArrayListImpl<A> extends ArrayList<A> {
   // Deletion of mid, next points to the next element (or past-the-end)
   method Erase(mid: ListIterator<A>) returns (next: ListIterator<A>)
     modifies this, Repr()
+    requires allocated(Repr())
+
     requires Valid()
     requires mid.Valid()
     requires mid.Parent() == this
-    requires mid.HasNext()
+    requires mid.HasNext?()
     requires mid in Iterators()
-    requires forall x | x in Repr() :: allocated(x)
-    
     ensures Valid()
     ensures Model() == Seq.Remove(old(Model()), old(mid.Index()))
 
-    ensures forall x {:trigger x in Repr(), x in old(Repr())} | x in Repr() - old(Repr()) :: fresh(x)
     ensures fresh(Repr() - old(Repr()))
-    ensures forall x | x in Repr() :: allocated(x)
+    ensures allocated(Repr())
 
     ensures fresh(next)
-    ensures Iterators() == {next} + old(Iterators())
-    ensures forall it | it in old(Iterators()) && old(it.Valid()) && old(it.HasNext())
-      :: it.Valid() && old(it.Parent()) == it.Parent() && old(it.Index()) == it.Index();    
-    ensures next.Valid() && next.Parent() == this && next.Index() == mid.Index();
+    ensures Iterators() >= {next} + old(Iterators())
+    ensures next.Valid() && next.Parent() == this && next.Index() == old(mid.Index())
+     ensures forall it | it in old(Iterators()) && old(it.Valid()) && old(it.HasNext?())
+      :: it.Valid() && it.Parent() == old(it.Parent()) && it.Index() == old(it.Index())
   {
     var midImpl := mid as ArrayListIteratorImpl;
     assert midImpl.index == mid.Index();
